ViewsProof.v
@@ -5,91 +5,6 @@ From Views Require Import ViewFunctions.
 Require Import PeanoNat.
 
 
-Proposition to_view_injective :
-  forall n, Injective (to_view n).
-Proof.
-  unfold Injective.
-  split.
-  intros.
-  unfold to_view in H.
-  apply to_nat_injective in H.
-  apply H.
-  intro. apply I.
-Qed.
-
-Proposition reverse_preserves_injectivity :
-  forall T n (v : ViewArray[[T;n]]), Injective v -> Injective (reverse v).
-Proof.
-  unfold Injective.
-  intros.
-  destruct H.
-  unfold reverse in *.
-  split.
-  - intros. apply H in H1.
-  destruct x,y.
-  inversion H1.
-  apply sub_injective with (c := n-1) in H5.
-  subst. apply unif_Idx.
-  destruct n. inversion H2. simpl. rewrite Nat.sub_0_r. apply le_S_n. apply H2.
-  destruct n. inversion H3. simpl. rewrite Nat.sub_0_r. apply le_S_n. apply H3.
-  - intros. apply H0.
-Qed.
-
-Proposition select_preserves_injectivity :
-  forall T n (a : nat) (b : nat) (v : ViewArray[[T;b+n]]), Injective v -> Injective (select a b v).
-Proof.
-  unfold Injective.
-  intros.
-  split.
-  - intros. destruct H. unfold select in H0.
-  apply H in H0.
-  inversion H0.
-  apply add_injective in H3.
-  apply to_nat_injective in H3.
-  apply H3.
-  - intros. apply H.
-Qed.
-
-Proposition transpose_preserves_injectivity :
-  forall T n m (v : ViewArray[[[[T;n]];m]]), Injective v -> Injective (transpose v).
-Proof.
-  unfold Injective.
-  split.
-  - intros.
-  unfold transpose in H0.
-  apply FunOverlap in H0.
-  destruct H0.
-  destruct H0.
-  assert (v x0 = v x1).
-  apply FunOverlap. exists x. exists y. apply H0. apply H in H1. subst.
-  destruct H.
-  destruct H1 with (i := x1).
-  apply H2 in H0. apply H0.
-  - intros. split.
-    + destruct H. intros. unfold transpose in H1.
-  assert (v x = v y). apply FunOverlap. exists i,i. apply H1. apply H in H2. apply H2.
-    + destruct H. intro. unfold transpose. destruct H0 with (i := i0).
-  apply H2.
-Qed.
-
-Proposition group_preserves_injectivity :
-  forall T n m (v : ViewArray[[T;m*n]]), Injective v -> Injective (group m v).
-Proof.
-  unfold Injective.
-  intros.
-  destruct H.
-  split.
-  - intros. unfold group in H1.
-  apply FunOverlap in H1. destruct H1. destruct H1. apply H in H1.
-  inversion H1. apply projection_injective in H3. injection H3. intros. apply to_nat_injective in H2. apply H2.
-  apply BoundedInt. apply BoundedInt.
-  - split.
-    + intros. unfold group in H1. apply H in H1.
-    inversion H1. apply projection_injective in H3. injection H3. intro. apply to_nat_injective in H2. apply H2.
-    apply BoundedInt. apply BoundedInt.
-    + intro. unfold group. apply H0.
-Qed.
-
 Fixpoint cat {T : Type} (A : List T) (B : List T) : List T :=
   match A with
   | [] => B
@@ -98,10 +13,23 @@ end.
 
 Notation "A ++ B" := (cat A B).
 
+
+Fixpoint tupcat {A : List nat} {B : List nat} : Tuple A -> Tuple B -> Tuple (A++B) :=
+  match A with
+  | [] => fun (_ : Tuple []) (y : Tuple B) => y
+  | A => fun (x : Tuple A) (y : Tuple B) => match x with | (i,x) => (i,tupcat x y) end
+end.
+
 Fixpoint curry_partialApp {A : List nat} {B : List nat} : ViewArray (A++B) -> Tuple A -> ViewArray B :=
   match A with
   | [] => fun (v : ViewArray ([]++B)) (x : Tuple []) => v
   | A => fun (v : ViewArray (A++B)) (x : Tuple A) => match x with | (x,y) => curry_partialApp (v x) y end
+end.
+
+Fixpoint curry_totalApp {A : List nat} : ViewArray A -> Tuple A -> nat :=
+  match A with
+  | [] => fun (v : ViewArray []) (x : Tuple []) => v
+  | A => fun (v : ViewArray A) (x : Tuple A) => match x with | (x,y) => curry_totalApp (v x) y end
 end.
 
 Fixpoint reorder {C : List nat} {n : nat} {A : List nat}  : ViewArray (C++[[A;n]]) ->  ViewArray [[C++A;n]] :=
@@ -109,6 +37,107 @@ Fixpoint reorder {C : List nat} {n : nat} {A : List nat}  : ViewArray (C++[[A;n]
   | [] => fun (v : ViewArray ([]++[[A;n]])) x => v x
   | C => fun (v : ViewArray (C++[[A;n]])) x => fun i => reorder (v i) x
 end.
+
+Definition Injective {A : List nat} (v : ViewArray A) : Prop :=
+  forall x y, (curry_totalApp v x) = (curry_totalApp v y) -> x = y.
+
+
+Definition preserveInjectivity {A : List nat} {B : List nat} (f : ViewArray A -> ViewArray B) :=
+  forall (C : List nat) (v : ViewArray (C++A)),
+  Injective v ->
+  (forall (i j : Tuple C) (x y : Tuple B),
+  curry_totalApp (f (curry_partialApp v i)) x = curry_totalApp (f (curry_partialApp v j)) y -> i = j /\ x = y).
+
+Proposition preserveInjectivity_is_correct :
+  forall A B (f : ViewArray A -> ViewArray B), preserveInjectivity f -> (forall v, Injective v -> Injective (f v)).
+Proof.
+  unfold preserveInjectivity.
+  intros.
+  unfold Injective.
+  intros.
+  apply H with (C := Nil nat) (x := x) (y := y) (i := I) (j := I) in H0.
+  destruct H0.
+  apply H2.
+  simpl. apply H1.
+Qed.
+
+Proposition to_view_injective :
+  forall n, Injective (to_view n).
+Proof.
+  unfold Injective.
+  intros.
+  unfold to_view in H.
+  simpl in H.
+  destruct x,y.
+  apply to_nat_injective in H.
+  destruct t,t0.
+  rewrite H.
+  reflexivity.
+Qed.
+
+Proposition reverse_preserves_injectivity :
+  forall T n (v : ViewArray[[T;n]]), Injective v -> Injective (reverse v).
+Proof.
+  unfold Injective.
+  intros.
+  unfold reverse in *.
+  destruct x as [x tx],y as [y ty].
+  simpl in *.
+  apply H with (x := ((Id n (n - 1 - to_nat x) reverseProof),tx)) (y := ((Id n (n - 1 - to_nat y) reverseProof),ty)) in H0.
+  injection H0.
+  intros.
+  apply sub_injective in H2.
+  apply to_nat_injective in H2. subst. reflexivity.
+  destruct n. destruct x. inversion H3. simpl. rewrite Nat.sub_0_r. apply le_S_n. apply BoundedInt.
+  destruct n. destruct y. inversion H3. simpl. rewrite Nat.sub_0_r. apply le_S_n. apply BoundedInt.
+Qed.
+
+Proposition select_preserves_injectivity :
+  forall T n (a : nat) (b : nat) (v : ViewArray[[T;b+n]]), Injective v -> Injective (select a b v).
+Proof.
+  unfold Injective.
+  intros.
+  unfold select in H0.
+  simpl in H0.
+  destruct x as [x tx],y as [y ty].
+  apply H with (x := ((Id (b + n) (a + to_nat x) selectProof),tx)) (y := ((Id (b + n) (a + to_nat y) selectProof),ty)) in H0.
+  injection H0. intros.
+  apply add_injective in H2.
+  apply to_nat_injective in H2.
+  subst. reflexivity.
+Qed.
+
+Proposition transpose_preserves_injectivity :
+  forall T n m (v : ViewArray[[[[T;n]];m]]), Injective v -> Injective (transpose v).
+Proof.
+  unfold Injective.
+  intros.
+  unfold transpose in *.
+  destruct x as [ix tx], y as [iy ty], tx as [jx tx], ty as [jy ty].
+  simpl in *.
+  apply H with (x := (jx,(ix,tx))) (y := (jy,(iy,ty))) in H0.
+  injection H0.
+  intros.
+  subst. reflexivity.
+Qed.
+
+Proposition group_preserves_injectivity :
+  forall T n m (v : ViewArray[[T;m*n]]), Injective v -> Injective (group m v).
+Proof.
+  unfold Injective.
+  intros.
+  unfold group in *.
+  destruct x as [ix tx], y as [iy ty], tx as [jx tx], ty as [jy ty].
+  simpl in *.
+  apply H with (x := ((Id (m * n) (to_nat jx + m * to_nat ix) groupProof),tx)) (y := ((Id (m * n) (to_nat jy + m * to_nat iy) groupProof),ty)) in H0.
+  inversion H0.
+  apply projection_injective in H2.
+  inversion H2.
+  apply to_nat_injective in H4, H5.
+  subst. reflexivity.
+  apply BoundedInt.
+  apply BoundedInt.
+Qed.
 
 Lemma reorder_is_correct :
   forall C A (n : nat) (v : ViewArray (C++(n::A))) (i : Tuple C) (x : Idx n),
@@ -123,19 +152,112 @@ Proof.
   rewrite H. simpl. reflexivity.
 Qed.
 
-Definition preserveInjectivity {A : List nat} {B : List nat} (f : ViewArray A -> ViewArray B) :=
-  forall (C : List nat) (v : ViewArray (C++A)),
-  Injective v ->
-      (forall i : Tuple C, Injective (f (curry_partialApp v i)))
-      /\ (forall i j : Tuple C, f (curry_partialApp v i) = f (curry_partialApp v j) -> i = j).
-
-Proposition preserveInjectivity_preserves_injectivity :
-  forall A B (f : ViewArray A -> ViewArray B), preserveInjectivity f -> (forall v, Injective v -> Injective (f v)).
+Lemma reorder_is_correct_2 :
+  forall C A (n : nat) (v : ViewArray (C++(n::A))) (i : Tuple C) (x : Idx n),
+  curry_partialApp (reorder v x) i = curry_partialApp v i x.
 Proof.
-  unfold preserveInjectivity.
   intros.
-  apply H with (C := Nil nat) in H0.
-  destruct H0. simpl in H0. apply H0. apply I.
+  induction C.
+  - simpl. reflexivity.
+  - destruct i. simpl.
+  apply IHC.
+Qed.
+
+Lemma decomposition :
+  forall C A (v : ViewArray (C++A)) (x : Tuple (C++A)),
+  exists (i : Tuple C) (j : Tuple A),
+  curry_totalApp v x = curry_totalApp (curry_partialApp v i) j /\ x = (tupcat i j).
+Proof.
+  intros.
+  induction C.
+  - simpl in *. exists I,x. split; reflexivity.
+  - simpl. destruct x.
+  assert (exists (i0 : Tuple C) (j : Tuple A),
+        curry_totalApp (v i) t = curry_totalApp (curry_partialApp (v i) i0) j /\ t = tupcat i0 j).
+  apply IHC.
+  destruct H.
+  destruct H.
+  exists (i,x).
+  exists x0.
+  split.
+  apply H.
+  assert (t = tupcat x x0). apply H.
+  subst. reflexivity.
+Qed.
+
+Lemma recomposition :
+  forall C A (v : ViewArray (C++A)) (i : Tuple C) (j : Tuple A),
+  curry_totalApp v (tupcat i j) = curry_totalApp (curry_partialApp v i) j.
+Proof.
+  induction C.
+  - intros. destruct i. simpl in *. reflexivity.
+  - intros. destruct i as [i ti].
+    simpl in *. apply IHC.
+Qed.
+
+Lemma tupcat_injective :
+  forall A B (x1 x2 : Tuple A) (y1 y2 : Tuple B),
+  tupcat x1 y1 = tupcat x2 y2 -> (x1,y1) = (x2,y2).
+Proof.
+  intros.
+  induction A.
+  - destruct x1,x2. simpl in H. subst. reflexivity.
+  - destruct x1 as [x1 tx1],x2 as [x2 tx2].
+  simpl in H.
+  injection H. intros. apply IHA in H0. inversion H0. subst. reflexivity.
+Qed.
+
+Proposition reorder_keeps_injectivity :
+  forall C A (n : nat) (v : ViewArray (C++(n::A))),
+  Injective v -> Injective (reorder v).
+Proof.
+  intros C A.
+  destruct C.
+  - intros. simpl in *. unfold Injective in *.
+    intros. simpl in *.
+    apply H in H0.
+    apply H0.
+  - unfold Injective.
+    intros.
+    destruct x as [x1 tx],y as [y1 ty].
+    destruct tx as [x2 tx], ty as [y2 ty].
+    assert (Hx:exists (i : Tuple (n::h::C)) (j : Tuple A),
+    curry_totalApp (reorder v) (x1, (x2, tx)) = curry_totalApp (curry_partialApp (reorder v) (A := n::h::C) i) j
+    /\ (x1,(x2,tx)) = tupcat i j).
+    apply decomposition.
+    destruct Hx as [ix Hx]. destruct Hx as [jx Hx].
+    simpl in *.
+    destruct ix as [ix1 tix].
+    destruct tix as [ix2 tix].
+    destruct Hx as [Hx Hi].
+    rewrite reorder_is_correct_2 in Hx.
+    rewrite Hx in H0.
+    assert (Hy:exists (i : Tuple (n::h::C)) (j : Tuple A),
+    curry_totalApp (reorder v (C:=h::C)) (y1, (y2, ty)) = curry_totalApp (curry_partialApp (reorder v (C := h::C)) (A := n::h::C) i) j
+    /\ (y1,(y2,ty)) = tupcat i j).
+    apply decomposition.
+    destruct Hy as [iy Hy]. destruct Hy as [jy Hy].
+    simpl in *.
+    destruct iy as [iy1 tiy].
+    destruct tiy as [iy2 tiy].
+    destruct Hy as [Hy Hj].
+    rewrite reorder_is_correct_2 in Hy.
+    rewrite Hy in H0.
+    assert (curry_totalApp (curry_partialApp v (A := (h::C)) (ix2,tix)) (ix1,jx) = curry_totalApp v (A := ((h::C)++(n::A))) (tupcat (ix2,tix) (A:=(h::C)) (ix1,jx) (B:=(n::A)))).
+    symmetry. apply recomposition with (i := (ix2,tix)) (j := (ix1,jx)).
+    simpl in H1. rewrite H1 in H0.
+    assert (curry_totalApp (curry_partialApp v (A := (h::C)) (iy2,tiy)) (iy1,jy) = curry_totalApp v (A := ((h::C)++(n::A))) (tupcat (iy2,tiy) (A:=(h::C)) (iy1,jy) (B:=(n::A)))).
+    symmetry. apply recomposition with (i := (iy2,tiy)) (j := (iy1,jy)).
+    simpl in H2. rewrite H2 in H0.
+    rewrite Hi,Hj.
+    apply H with (x := (ix2,tupcat tix (ix1,jx) (B := (n::A)))) (y := (iy2,tupcat tiy (iy1,jy) (B := (n::A)))) in H0.
+    injection H0.
+    intros.
+    apply tupcat_injective in H3.
+    injection H3.
+    intros.
+    subst.
+    reflexivity.
 Qed.
 
 Proposition curry_partialApp_keeps_injectivity :
@@ -144,50 +266,69 @@ Proof.
   intros A B.
   induction A.
   + simpl. intros. apply H.
-  + intros. destruct H. intros. simpl. destruct i.
-      assert (Injective (v i)). apply H0.
-      apply IHA with (i := t) in H1.
-      apply H1.
+  + intros. intros. simpl. destruct i.
+      assert (Injective (v i)). {
+        unfold Injective.
+        intros. assert ((i,x) = (i,y)).
+        apply H. apply H0. injection H1. trivial.
+      }
+      apply IHA with (i := t) in H0.
+      apply H0.
 Qed.
 
-Lemma reorder_keeps_injectivity :
-  forall C A (n : nat) (v : ViewArray (C++(n::A))),
-  Injective v -> Injective (reorder v).
+
+Lemma lemma1 :
+  forall A B (v : ViewArray (A++B)),
+  Injective v -> (forall (i j : Tuple A) (x y : Tuple B), (curry_totalApp (curry_partialApp v i) x) = (curry_totalApp (curry_partialApp v j) y)-> i = j /\ x = y).
 Proof.
   intros.
-  unfold Injective.
-  split.
-  - intros.
-    induction C.
-    + simpl in H0. apply H. apply H0.
-Admitted.
-
-
-Proposition curry_partialApp_injective :
-  forall A B (v : ViewArray (A++B)), Injective v -> (forall i j, (curry_partialApp v i) = (curry_partialApp v j) -> i = j).
-Proof.
-  intros A B.
-  induction A.
-  - destruct i,j. reflexivity.
-  - destruct i,j. intros. destruct H.
-    simpl in *.
-    
-Admitted.
+  destruct A.
+  - destruct i,j. simpl in H0. apply H in H0. split. reflexivity. apply H0.
+  - destruct i as [i ti],j as [j tj].
+  simpl in H0.
+  assert (curry_totalApp (curry_partialApp (v i) ti) x = curry_totalApp v (tupcat (i,ti) (A := (h::A)) x)).
+  symmetry. apply recomposition with (i := (i,ti)).
+  assert (curry_totalApp (curry_partialApp (v j) tj) y = curry_totalApp v (tupcat (j,tj) (A := (h::A)) y)).
+  symmetry. apply recomposition with (i := (j,tj)).
+  rewrite H1,H2 in H0.
+  apply H in H0.
+  apply tupcat_injective in H0.
+  injection H0.
+  intros. subst. split;reflexivity.
+Qed.
 
 Proposition reverse_preserves_injectivity2 :
   forall T n, preserveInjectivity reverse (A := (n::T)).
 Proof.
   unfold preserveInjectivity.
   intros.
-  split.
-  - intro i. apply curry_partialApp_keeps_injectivity with (i := i) in H.
-  apply reverse_preserves_injectivity in H. apply H.
-  - intros. unfold reverse in H0. apply FunOverlap in H0.
-    destruct H0; destruct H0.
-    assert (curry_partialApp v i = curry_partialApp v j).
-    apply FunOverlap. exists (Id n (n - 1 - to_nat x) reverseProof), (Id n (n - 1 - to_nat x0) reverseProof).
-    apply H0.
-    apply curry_partialApp_injective with (i := i) (j := j) in H. apply H. apply H1.
+  unfold reverse in H0.
+  destruct x as [x tx],y as [y ty].
+  simpl in H0.
+  destruct C.
+  - simpl in *. unfold Injective in H.
+    apply H with (x := ((Id n (n - 1 - to_nat x) reverseProof),tx)) (y := ((Id n (n - 1 - to_nat y) reverseProof),ty)) in H0.
+    inversion H0.
+    apply sub_injective in H2.
+    apply to_nat_injective in H2. subst. destruct i,j. split; reflexivity.
+    destruct n. destruct x. inversion H1. simpl. rewrite Nat.sub_0_r. apply le_S_n. apply BoundedInt.
+    destruct n. destruct y. inversion H1. simpl. rewrite Nat.sub_0_r. apply le_S_n. apply BoundedInt.
+  - destruct i as [i ti],j as [j tj].
+    set (i' := (i,ti)) in *.
+    set (x' := ((Id n (n - 1 - to_nat x) reverseProof),tx)) in *.
+    set (j' := (j,tj)) in *.
+    set (y' := ((Id n (n - 1 - to_nat y) reverseProof),ty)) in *.
+    assert ((curry_totalApp (curry_partialApp v i') x') = (curry_totalApp (curry_partialApp v j') y')-> i' = j' /\ x' = y').
+    apply lemma1. apply H.
+    simpl in *.
+    apply H1 in H0. destruct H0.
+    unfold x',y' in H2.
+    inversion H2.
+    apply sub_injective in H4.
+    apply to_nat_injective in H4.
+    unfold i',j' in *. inversion H0. subst. split; reflexivity.
+    destruct n. destruct x. inversion H3. simpl. rewrite Nat.sub_0_r. apply le_S_n. apply BoundedInt.
+    destruct n. destruct y. inversion H3. simpl. rewrite Nat.sub_0_r. apply le_S_n. apply BoundedInt.
 Qed.
 
 Proposition select_preserves_injectivity2 :
@@ -195,15 +336,30 @@ Proposition select_preserves_injectivity2 :
 Proof.
   unfold preserveInjectivity.
   intros.
-  split.
-  - intro i. apply curry_partialApp_keeps_injectivity with (i := i) in H.
-  apply select_preserves_injectivity with (a := a) in H. apply H.
-  - intros. unfold select in H0. apply FunOverlap in H0.
-    destruct H0; destruct H0.
-    assert (curry_partialApp v i = curry_partialApp v j).
-    apply FunOverlap. exists (Id (b + n) (a + to_nat x) selectProof), (Id (b + n) (a + to_nat x0) selectProof).
-    apply H0.
-    apply curry_partialApp_injective with (i := i) (j := j) in H. apply H. apply H1.
+  destruct x as [x tx],y as [y ty].
+  destruct C.
+  - unfold select in *.
+    unfold Injective in H.
+    apply H with (x := ((Id (b + n) (a + to_nat x) selectProof),tx)) (y := ((Id (b + n) (a + to_nat y) selectProof),ty)) in H0.
+    inversion H0.
+    apply add_injective in H2.
+    apply to_nat_injective in H2.
+    subst. destruct i,j. split;reflexivity.
+  - destruct i as [i ti],j as [j tj].
+    set (i' := (i,ti)) in *.
+    set (x' := ((Id (b + n) (a + to_nat x) selectProof),tx)) in *.
+    set (j' := (j,tj)) in *.
+    set (y' := ((Id (b + n) (a + to_nat y) selectProof),ty)) in *.
+    assert ((curry_totalApp (curry_partialApp v i') x') = (curry_totalApp (curry_partialApp v j') y')-> i' = j' /\ x' = y').
+    apply lemma1. apply H.
+    unfold x',y',i',j' in *.
+    apply H1 in H0.
+    destruct H0.
+    injection H0. intros.
+    inversion H2.
+    apply add_injective in H6.
+    apply to_nat_injective in H6.
+    subst. split;reflexivity.
 Qed.
 
 Proposition transpose_preserves_injectivity2 :
@@ -211,18 +367,26 @@ Proposition transpose_preserves_injectivity2 :
 Proof.
   unfold preserveInjectivity.
   intros.
-  split.
-  - intro i. apply curry_partialApp_keeps_injectivity with (i := i) in H.
-  apply transpose_preserves_injectivity in H. apply H.
-  - intros. unfold transpose in H0. apply FunOverlap in H0.
-    destruct H0; destruct H0.
-    apply FunOverlap in H0.
-    destruct H0; destruct H0.
-    assert (curry_partialApp v i = curry_partialApp v j).
-    apply FunOverlap. exists x1,x2.
-    apply FunOverlap. exists x,x0.
-    apply H0.
-    apply curry_partialApp_injective with (i := i) (j := j) in H. apply H. apply H1.
+  destruct C.
+  - destruct i,j,x as [xi tx], y as [yi ty], tx as [xj tx], ty as [yj ty]. unfold Injective in H.
+    simpl in *.
+    apply H with (x := (xj,(xi,tx))) (y := (yj,(yi,ty))) in H0.
+    injection H0.
+    intros.
+    subst. split;reflexivity.
+  - destruct i as [i ti],j as [j tj].
+    destruct x as [xi tx], y as [yi ty], tx as [xj tx], ty as [yj ty].
+    set (i' := (i,ti)) in *.
+    set (x' := (xj,(xi,tx))) in *.
+    set (j' := (j,tj)) in *.
+    set (y' := (yj,(yi,ty))) in *.
+    assert ((curry_totalApp (curry_partialApp v i') x') = (curry_totalApp (curry_partialApp v j') y')-> i' = j' /\ x' = y').
+    apply lemma1. apply H.
+    unfold x',y',i',j' in *.
+    apply H1 in H0.
+    destruct H0.
+    injection H0. injection H2. intros. subst.
+    split;reflexivity.
 Qed.
 
 Proposition group_preserves_injectivity2 :
@@ -230,50 +394,87 @@ Proposition group_preserves_injectivity2 :
 Proof.
   unfold preserveInjectivity.
   intros.
-  split.
-  - intro i. apply curry_partialApp_keeps_injectivity with (i := i) in H.
-  apply group_preserves_injectivity in H. apply H.
-  - intros. unfold group in H0. apply FunOverlap in H0.
-    destruct H0; destruct H0.
-    apply FunOverlap in H0.
-    destruct H0; destruct H0.
-    assert (curry_partialApp v i = curry_partialApp v j).
-    apply FunOverlap. exists (Id (m * n) (to_nat x1 + m * to_nat x) groupProof),(Id (m * n) (to_nat x2 + m * to_nat x0) groupProof).
-    apply H0.
-    apply curry_partialApp_injective with (i := i) (j := j) in H. apply H. apply H1.
+  destruct C.
+  - destruct i,j,x as [xi tx], y as [yi ty], tx as [xj tx], ty as [yj ty]. unfold Injective in H.
+    unfold group in H0.
+    simpl in *.
+    apply H with
+      (x := (Id (m * n) (to_nat xj + m * to_nat xi) groupProof,tx))
+      (y := (Id (m * n) (to_nat yj + m * to_nat yi) groupProof,ty))
+     in H0.
+    inversion H0.
+    apply projection_injective in H2.
+    injection H2.
+    intros.
+    apply to_nat_injective in H1,H4.
+    subst. split;reflexivity.
+    apply BoundedInt.
+    apply BoundedInt.
+  - destruct i as [i ti],j as [j tj],x as [xi tx], y as [yi ty], tx as [xj tx], ty as [yj ty].
+  set (i' := (i,ti)) in *.
+  set (x' := (Id (m * n) (to_nat xj + m * to_nat xi) groupProof,tx)) in *.
+  set (j' := (j,tj)) in *.
+  set (y' := (Id (m * n) (to_nat yj + m * to_nat yi) groupProof,ty)) in *.
+  assert ((curry_totalApp (curry_partialApp v i') x') = (curry_totalApp (curry_partialApp v j') y')-> i' = j' /\ x' = y').
+  apply lemma1. apply H.
+  apply H1 in H0.
+  unfold i',j',x',y' in *.
+  destruct H0.
+  injection H0.
+  inversion H2.
+  apply projection_injective in H4.
+  inversion H4.
+  apply to_nat_injective in H6,H7.
+  intros. subst. split;reflexivity.
+  apply BoundedInt.
+  apply BoundedInt.
 Qed.
+
 
 Proposition map_preserves_injectivity :
   forall A B (n : nat) (f : ViewArray A -> ViewArray B), preserveInjectivity f -> preserveInjectivity (map f (n := n)).
 Proof.
+  unfold preserveInjectivity.
   intros.
-  unfold preserveInjectivity in H.
-  split; set (v' := reorder v).
-  - assert (Injective v'). apply reorder_keeps_injectivity. apply H0.
-    unfold map. intros. simpl. split.
-    + intros.
-    apply H with (C := (n::C)) in H1.
+  destruct C.
+  - destruct i,j,x as [xi tx], y as [yi ty].
+    simpl in *.
+    unfold map in H1.
+    assert (curry_totalApp (f (curry_partialApp v (A := (n::[])) (xi,I))) tx = curry_totalApp (f (curry_partialApp v (A := (n::[])) (yi,I))) ty ->
+      (xi,I) = (yi,I) /\ tx = ty).
+    apply H with (i := (xi,I)) (j := (yi,I)).
+    apply H0.
+    simpl in H2.
+    apply H2 in H1.
     destruct H1.
-    assert (curry_partialApp v i x = curry_partialApp v' (A := (n::C)) (x,i)). apply reorder_is_correct.
-    assert (curry_partialApp v i y = curry_partialApp v' (A := (n::C)) (y,i)). apply reorder_is_correct.
-    rewrite H4 in H2. rewrite H5 in H2.
-    apply H3 in H2.
-    injection H2. trivial.
-    + intros. unfold preserveInjectivity in H.
-    apply H with (C := (n::C)) in H1.
+    injection H1.
+    intros.
+    subst.
+    split;reflexivity.
+  - destruct i as [i ti],j as [j tj],x as [xi tx], y as [yi ty].
+    unfold map in *.
+    set (v' := reorder v (C := (h::C))).
+    assert (curry_partialApp v (A := (h::C)) (i,ti) xi = curry_partialApp (reorder v (C := (h::C))) (A := (n::h::C)) (xi,(i,ti))).
+    apply reorder_is_correct.
+    assert (curry_partialApp v (A := (h::C)) (j,tj) yi = curry_partialApp (reorder v (C := (h::C))) (A := (n::h::C)) (yi,(j,tj))).
+    apply reorder_is_correct.
+    simpl in *.
+    rewrite H2 in H1.
+    rewrite H3 in H1.
+    set (i' := (xi,(i,ti))) in *.
+    set (x' := tx) in *.
+    set (j' := (yi,(j,tj))) in *.
+    set (y' := ty) in *.
+    assert (curry_totalApp (f (curry_partialApp (reorder v (C := (h::C))) (A := (n::h::C)) i')) x' = curry_totalApp (f (curry_partialApp (reorder v (C := (h::C))) (A := (n::h::C)) j')) y' ->
+    i' = j' /\ x' = y').
+    apply H.
+    apply reorder_keeps_injectivity.
+    apply H0.
+    unfold i',j',x',y' in *.
+    apply H4 in H1.
     destruct H1.
-    assert (curry_partialApp v i i0 = curry_partialApp v' (A := (n::C)) (i0,i)). apply reorder_is_correct.
-    rewrite H3.
-    apply H1.
-  - assert (Injective v'). apply reorder_keeps_injectivity. apply H0.
-  unfold map.
-  intros. apply H with (C := (n::C)) in H1.
-  simpl in *.
-  destruct H1.
-  assert (forall x, curry_partialApp v i x = curry_partialApp v' (A := (n::C)) (x,i)). apply reorder_is_correct.
-  assert (forall x, curry_partialApp v j x = curry_partialApp v' (A := (n::C)) (x,j)). apply reorder_is_correct.
-  apply FunOverlap in H2. destruct H2. destruct H2.
-  rewrite H4 with (x := x) in H2. rewrite H5 with (x := x0) in H2.
-  simpl in H2.
-  apply H3 with (i := (x,i)) (j := (x0,j)) in H2. injection H2. intros. apply H6.
+    injection H1.
+    intros.
+    subst.
+    split;reflexivity.
 Qed.
